

Linear regression

- [1 Notation](#)
- [2 Least square estimation](#)
 - [2.1 Mean square error and least square solution](#)
 - [2.2 Best model as projection](#)
 - [2.3 Risk decomposition](#)
 - [2.4 Trade-off between variance and bias](#)
 - [2.5 Asymptotic properties of ordinary least square](#)
- [3 Ridge regression](#)
 - [3.1 Ridge regression as constrained optimization](#)
 - [3.2 Ridge regression as MAP](#)
 - [3.3 Ridge regression as weighted projection](#)
 - [3.4 Ridge regression as dropout](#)
 - [3.5 Ridge regression as noises addition](#)
- [4 Lasso](#)
 - [4.1 Sparse parttern of lasso solution](#)
 - [4.2 Lasso and robustness](#)
- [5 Appendix](#)
 - [5.1 Appendix-1](#)
 - [5.2 Appendix-2](#)
 - [5.3 Appendix-3](#)
 - [5.4 Appendix-4](#)
 - [5.5 Appendix-5](#)
 - [5.6 Appendix-6](#)

Notation

We will use operator notation. Typically, P is used to represent expectation over distribution p :

$$Pf(X) = \int f(x)p(x)dx.$$

For example, if we use \mathbb{P}_n to denote empirical density, then

$$\mathbb{P}_n f(X) = \int f(x) \frac{1}{N} \sum_i \delta(x - x_i) dx = \frac{1}{N} \sum_i f(x_i).$$

We will use \mathbb{E} to represent average over all the randomness.

X is usually denoted as random variable (predictors) and \mathbb{X} is denoted as design matrix.

Least square estimation

Mean square error and least square solution

The least square estimation is a decision criterion based on L2 risk (mean square error):

$$f^* = \arg \min_f P(Y - f(X))^2,$$

where X is predictor and Y is response. This criterion may stem from the MLE based on Gaussian conditional mean assumption, but anyway we will use this criterion without any assumption. By conditioning on X , we can find the best estimation that minimizes L2 risk is exactly conditional mean (see [Appendix-1](#)):

$$f^*(X) = P(Y|X).$$

In linear regression, we restrict to linear functions $f(x) = \beta^T x$, so we only search through linear function space:

$$\beta^* = \arg \min_{\beta} P(Y - \beta^T X)^2.$$

Assume PXX^T is positive definite (thus invertible), then the problem above is a convex optimization and we easily find β^* by letting its gradient be zero:

$$PXX^T \beta^* = P(XY) \Rightarrow \beta^* = (PXX^T)^{-1} PXY.$$

This is also called the **normal equation**. Essentially $\hat{Y} = (\beta^*)^T X$ is the **best linear estimator** we can find. It is shown that $(\beta^*)^T X$ is actually the projection of conditional mean $f^*(X) = P(Y|X)$ onto linear function space (see [Appendix-2](#)).

Here comes the problem. Since we do not know distribution P , so in fact we can only estimate β^* . The estimation $\hat{\beta}_n$ is defined by empirical risk minimizer (ERM):

$$\hat{\beta}_n = \arg \min_{\beta} \mathbb{P}_n(Y - \beta^T X)^2.$$

Similarly, we obtain the normal equation for empirical least square estimation:

$$\mathbb{P}_n XX^T \hat{\beta}_n = \mathbb{P}_n XY \Rightarrow \hat{\beta}_n = (\mathbb{P}_n XX^T)^{-1} \mathbb{P}_n XY.$$

Best model as projection

There are some interesting facts we should know about the relations between regression function $P(Y|X)$ and best linear model $(\beta^*)^T X$.

Remark

The best linear model $(\beta^*)^T X$ is the **projection** of regression function $P(Y|X)$ onto linear function space. In ge

Proof

Note that we can decompose L2 risk into

Equation

$$P(Y - f(X))^2 = P(Y - P(Y|X) + P(Y|X) - f(X))^2 = P(\text{Var}\{Y|X\} + P(P(Y|X) - f(X))^2).$$

Equation

The first term has nothing to do with hypothesis space \mathcal{F} . So our best model in terms of L2 risk is

Equation

$$f^* = \arg \min_{f \in \mathcal{F}} P(Y - f(X))^2 = \arg \min_{f \in \mathcal{F}} P(P(Y|X) - f(X))^2.$$

Equation

It suggests we are actually projecting $P(Y|X)$ onto \mathcal{F} and get the best model.

Proof

Risk decomposition

The best model and $P(Y|X)$ are all independent of samples (data), and in practice the most ideal situation is that $\hat{\beta}_n \approx \beta^*$ (we cannot find $P(Y|X)$). To study the error of given $\hat{\beta}_n$, we can decompose its error into several parts:

$$\begin{aligned} E(Y - \hat{\beta}_n^T X)^2 &= P\text{Var}(Y|X) + E(P(Y|X) - \hat{\beta}_n^T X)^2 = \text{Noise} + E(P(Y|X) - (\beta^*)^T X + (\beta^*)^T X - \hat{\beta}_n^T X)^2 \\ &= \text{Noise} + P(P(Y|X) - (\beta^*)^T X)^2 + E((\beta^* - \hat{\beta}_n)^T X)^2 = \text{Noise} + \text{Appr. Err} + \text{Est. Err} \end{aligned}$$

where $\text{Noise} = P\text{Var}(Y|X)$ refers to noise in data, $\text{Appr. Err} = P(P(Y|X) - (\beta^*)^T X)^2$ is called **approximation error** that represents risk of our best model and $\text{Est. Err} = E((\beta^* - \hat{\beta}_n)^T X)^2$ is called **estimation error** that reflects the difference between our estimation and the best model. Only estimation error depends on our samples. The cross term is zero due to normal equation.

A typical trade-off here is between approximation error and estimation error. It depends on the size (complexity) of our hypothesis space. Consider two extreme cases: if we allow all kinds of possible functions, then definitely the approximation error would be zero, while the estimation error would be huge; on the contrary, if we only allow the simplest function (say, pre-determined constant prediction), then there would not be any estimation error, but the approximation error is large. In principle, estimation error would shrink as sample size grows, so a larger sample size allows a large hypothesis space.

Trade-off between variance and bias

Notice that estimation error can be further decomposed into the following:

$$E(X^T (\beta^* - \hat{\beta}_n))^2 = P(X^T E(\beta^* - \hat{\beta}_n)(\beta^* - \hat{\beta}_n)^T X).$$

Here $E(\beta^* - \hat{\beta}_n)(\beta^* - \hat{\beta}_n)^T$ is called **mean square error** of parameter estimation. It can be decomposed into bias and variance:

$$E(\beta^* - \hat{\beta}_n)(\beta^* - \hat{\beta}_n)^T = \text{Var}(\hat{\beta}_n) + (E\hat{\beta}_n - \beta^*)(E\hat{\beta}_n - \beta^*)^T.$$

As we can see latter, the idea of shrinkage method (regularization) is to increase bias a little but reduce variance a lot, which leads to the overall shrink of estimation error.

Asymptotic properties of ordinary least square

In this section, we are going to show that least square solution $\hat{\beta}_n$ will converge to best linear estimator β^* . Based on its asymptotical behavior, we can construct confidence interval for β^* .

To show this, consider the difference between them:

$$\begin{aligned}\hat{\beta}_n - \beta^* &= (\mathbb{P}_n XX^T)^{-1} \mathbb{P}_n XY - \beta^* = (\mathbb{P}_n XX^T)^{-1} \mathbb{P}_n X(Y - X^T \beta^*) \\ &= (\mathbb{P}_n XX^T)^{-1} (\mathbb{P}_n - P)X(Y - X^T \beta^*).\end{aligned}$$

The last line is due to normal equation $PX(Y - X^T \beta^*) = 0$. Now according to law of large number and central limit theorem,

$$\begin{aligned}\mathbb{P}_n XX^T &\rightarrow PXX^T \\ \sqrt{n}(\mathbb{P}_n - P)X(Y - X^T \beta^*) &\rightsquigarrow N(0, PXX^T(Y - X^T \beta^*)^2).\end{aligned}$$

So $\hat{\beta}_n \rightarrow \beta^*$ with

$$\sqrt{n}(\hat{\beta}_n - \beta^*) \rightsquigarrow N(0, \Sigma),$$

where $\Sigma = (PXX^T)^{-1} PXX^T (Y - X^T \beta^*)^2 (PXX^T)^{-1}$. In practice, we can estimate Σ using $\hat{\Sigma} = (\mathbb{P}_n XX^T)^{-1} \mathbb{P}_n XX^T (Y - X^T \hat{\beta}_n)^2 (\mathbb{P}_n XX^T)^{-1}$

Ridge regression

Notice that if linear model is correct, namely $P(Y|X) = X^T \beta^*$, then least square estimator $\hat{\beta}_n$ is unbiased because:

$$E\hat{\beta}_n = E(P_n XX)^{-1} P_n XY = E_X (P_n XX^T)^{-1} P_n X E_{Y|X} Y = E_X (P_n XX^T)^{-1} P_n XX^T \beta^* = \beta^*.$$

But as we can see in trade-off between variance and bias, it is not always a good idea to make a unbiased estimation if we want MSE to be lower. The idea of regularization is to significantly reduce estimation error through variance/bias trade-off, though approximation error may increase a little.

This motivates ridge regression. Ridge regression is defined as the following modified optimization problem:

$$\hat{\beta}_n = \arg \min_{\beta} \mathbb{P}_n (Y - X^T \beta)^2 + \lambda \|\beta\|_2^2.$$

It can be shown that this is definitely a convex problem given a positive λ . So the closed form solution for ridge regression is obtained by setting the gradient to zero:

$$\hat{\beta}_n = (\mathbb{P}_n XX^T + \lambda I)^{-1} \mathbb{P}_n XY.$$

There are plenty of ways to explain ridge regression.

Ridge regression as constrained optimization

We can prove that ridge regression (???) is equivalent to the following constrained optimization with certain $\lambda = \lambda(C)$:

$$\begin{aligned}\hat{\beta}_n &= \arg \min_{\beta} \mathbb{P}_n(Y - X^T \beta)^2, \\ \text{s.t. } \|\beta\|_2^2 &\leq C.\end{aligned}$$

This can be proved by using KKT conditions (see [Appendix-3](#)). It basically says that when doing ridge regression, we are actually doing least square but in a constrained hypothesis set. So intuitively the approximation error would be larger than OLS, since we have a smaller hypothesis space, but the estimation error would be (maybe) reduced. It had be shown that there exists some λ such that the mean square error of ridge is stricly less than OLS:

$$E\left\|\hat{\beta}_n^{\text{ridge}} - \beta^*\right\|_2^2 \leq E\left\|\hat{\beta}_n^{\text{OLS}} - \beta^*\right\|_2^2$$

Ridge regression as MAP

Another way to explain ridge is through Bayesian estimation. Suppose linear model is correct, that is $Y \sim N(X^T \beta, \sigma^2)$ and $\beta \sim N(0, \tau^2)$. To make a point estimation of β , we decide to maximize a posterior probability (MAP), that is

$$\hat{\beta}_n = \arg \min -\log p(\beta|\mathbb{X}, \mathbb{Y}) = \arg \min -\log p(\mathbb{Y}|\beta, \mathbb{X}) - \log p(\beta) = \arg \min_{\beta} \mathbb{P}_n(Y - X^T \beta)^2 +$$

So we can define $\sigma^2/n\tau^2 \triangleq \lambda$ as the regularization paramter. In practice, it is useful to first estimate $\hat{\sigma}^2/n\hat{\tau}^2$ as a initial value for λ . So in this point of view, ridge regression is just OLS plus the prior knowledge that each component of paramters β^* should be small and close to zero. This is why as a result we would shrink $\hat{\beta}_n$.

Ridge regression as weighted projection

Recall that least square prediction $\hat{\mathbb{Y}} = \mathbb{X}\hat{\beta}_n^{\text{OLS}}$, in terms of design matrix \mathbb{X} and response \mathbb{Y} , can be viewed as orthogonal projection of \mathbb{Y} onto range of \mathbb{X} :

$$\hat{\mathbb{Y}}^{\text{OLS}} = \mathbb{X}(\mathbb{X}\mathbb{X}^T)^{-1}\mathbb{X}^T\mathbb{Y} = \mathbb{U}\mathbb{U}^T\mathbb{Y} = \sum_j u_j u_j^T \mathbb{Y},$$

where $\mathbb{X} = \mathbb{U}\mathbb{D}\mathbb{V}^T$ is the SVD of design matrix. If we check the closed form solution of ridge, we find:

$$\hat{\mathbb{Y}}^{\text{ridge}} = \mathbb{X}(\mathbb{X}\mathbb{X}^T + \lambda I)^{-1}\mathbb{X}^T\mathbb{Y} = \sum_j u_j \text{diag}\left\{\frac{d_i^2}{d_i^2 + \lambda}\right\} u_j^T \mathbb{Y}.$$

So now we can clearly see how ridge regression shrinks the coefficients. Roughly speaking, the degree of shrinkage depends on the sample variance of features (or say principal components): if variance of certain is small, then we think it is unimportant and shrink it a lot.

Ridge regression as dropout

Dropout, that is to randomly zero out some components of predictors, is a common trick for regularization. We will show that dropout is equivalent to ridge regression. Consider the following formal definition of least square estimation with dropout:

$$\hat{\beta}_n = \arg \min_{\beta} \sum_k \sum_n (Y_n - (X_n \cdot Z_k)^T \beta / (1 - \phi))^2,$$

here Z_k are i.i.d. Bernulli vectors with $P(Z_{k,i} = 1) = 1 - \phi$. $X_n \cdot Z_k \triangleq (X_{n,1} Z_{k,1}, \dots, X_{n,p} Z_{k,p})$. Basically we create much more data by dropout. As we can create as much as dropout data we want, so

$$\hat{\beta}_n \approx \arg \min_{\beta} E_Z \mathbb{P}_n (Y - (X \cdot Z)^T \beta / (1 - \phi))^2,$$

Solving this optimization problem gives exactly the ridge regression

$$\hat{\beta}_n = (\mathbb{P}_n X X^T + \frac{\phi}{1 - \phi} \text{diag}\{\mathbb{P}_n X_i^2\})^{-1} \mathbb{P}_n X Y.$$

The proof is shown in [Appendix-4](#). Suppose each feature X_i is standardized, then dropout is the same as ridge regression in the sense that $\lambda = \phi / (1 - \phi)$.

Ridge regression as noises addition

Just as we can create data in case of dropout, we can also create data by adding noisy predictors. Let $W \sim N(0, \tau^2 I)$, then the noisy optimization problem becomes

$$\hat{\beta}_n = \arg \min_{\beta} E_W \mathbb{P}_n (Y - (X + W)^T \beta)^2.$$

By settin the gradient to zero, we find

$$\hat{\beta}_n = (\mathbb{P}_n X X^T + \tau^2 I)^{-1} \mathbb{P}_n X Y.$$

So our regularization parameter λ can be seen as the magnitude of noise τ^2 .

Lasso

Another shrinkage method is to apply L1 regularization:

$$\hat{\beta}_n = \arg \min_{\beta} \mathbb{P}_n (Y - X^T \beta)^2 + \lambda \|\beta\|_1.$$

Sparse parttern of lasso solution

As we all knew, lasso leads to sparsity. To see this, let us consider $\mathbb{P}_n X X^T = I$, then the lasso gives (see proof in [Appendix-5](#))

$$\hat{\beta}_n^{\text{lasso}} = \max(0, \hat{\beta}_n - \lambda/2),$$

where $\hat{\beta}_n$ is the OLS solution. We can see that lasso solution is sparse in the sense that its j^{th} component is zero if $(\hat{\beta}_n)_j < \lambda/2$.

Lasso and robustness

Another way to explain lasso is through robust regression, which is defined by the following:

$$\hat{\beta}_n = \arg \min_{\beta} \max_{\Delta \in M} \|\mathbb{Y} - (\mathbb{X} + \Delta)\beta\|_2,$$

where M is a set of matrix. To obtain lasso, let us consider a specific M , that is

$$M = \left\{ \Delta \mid \sqrt{\sum_i \Delta_{i,j}^2} \leq c_i \right\},$$

where $\{c_i\}$ is some constants. It can be shown that (see proof in [Appendix-6](#))

$$\max_{\Delta \in M} \|\mathbb{Y} - (\mathbb{X} + \Delta)\beta\|_2 = \|\mathbb{Y} - \mathbb{X}\beta\|_2 + \sum_i c_i |\beta_i|.$$

So the robust regression becomes exactly lasso (actually, square root of lasso since) if we let $c_i = \lambda$. The hyperparameter λ thus be can thought of the perturbation of design matrix.

Appendix

Appendix-1

To see the conditional mean is the best estimator that minimizes L2 risk, we first condition on X and get

$$P(Y - f(X))^2 = P(P(Y - P(Y|X) + P(Y|X) - f(X))^2 | X) = P(Y - P(Y|X))^2 + P(P(Y|X) - f(X))^2$$

then we can see that for each fixed X we should minimize

$$f^*(X) = \arg \min_a (P(Y|X) - f(X))^2 \Rightarrow f^*(X) = P(Y|X).$$

Appendix-2

Recall the definition of $\beta^* = \arg \min_{\beta} P(Y - \beta^T X)$. It turns out

$$P(Y - \beta^T X)^2 = P(Y - f^*(X) + f^*(X) - \beta^T X)^2 = P(Y - f^*(X))^2 + P(f^*(X) - \beta^T X)^2.$$

Thus we have

$$\beta^* = \arg \min_{\beta} P(f^*(X) - \beta^T X)^2,$$

which says $(\beta^*)^T X$ is the projection of conditional mean $f^*(X) = P(Y|X)$.

Appendix-3

The lagrangian of the constrained optimization (???) is

$$L(\beta, \lambda) = \mathbb{P}_n(Y - X^T \beta)^2 + \lambda(\|\beta\|_2^2 - C),$$

where λ is the lagrangian multiplier. Suppose λ^* is optimal solution of dual problem, then from KKT conditions we know that optimal solution $\hat{\beta}_n$ should be the minimizer of $L(\beta, \lambda^*)$, which is

$$\hat{\beta}_n = \arg \min_{\beta} \mathbb{P}_n(Y - X^T \beta)^2 + \lambda^* \|\beta\|_2^2.$$

For each C , we also solve a λ^* .

Appendix-4

Consider the gradient of dropout optimization:

$$\frac{\partial}{\partial \beta} E_Z \mathbb{P}_n(Y - (X \cdot Z)^T \beta / (1 - \phi))^2 = \frac{1}{1 - \phi} E_Z \mathbb{P}_n(Y - (X \cdot Z)^T \beta / (1 - \phi)) X \cdot Z = 0.$$

Notice that $E_Z X \cdot Z = X(1 - \phi)$ and $\mathbb{P}_n(X \cdot Z)(X \cdot Z)^T = XX^T + \frac{\phi}{1 - \phi} \text{diag}\{X_i^2\}$, getting

$$\mathbb{P}_n XY = \mathbb{P}_n XX^T + \frac{\phi}{1 - \phi} \text{diag}\{\mathbb{P}_n X_i^2\} \beta,$$

so

$$\hat{\beta}_n^{\text{dropout}} = \left(\mathbb{P}_n XX^T + \frac{\phi}{1 - \phi} \text{diag}\{\mathbb{P}_n X_i^2\} \right)^{-1} \mathbb{P}_n XY.$$

Appendix-5

Consider $\mathbb{P}_n XX^T = I$. Then since

$$\mathbb{P}_n(Y - X^T \beta)^2 = \mathbb{P}_n(Y - X^T \hat{\beta}_n + X^T \hat{\beta}_n - X^T \beta)^2 = \mathbb{P}_n Y^2 + \hat{\beta}_n^T \hat{\beta}_n + \|\hat{\beta}_n - \beta\|_2^2,$$

so the lasso becomes

$$\hat{\beta}_n^{\text{lasso}} = \arg \min_{\beta} \|\hat{\beta}_n - \beta\|_2^2 + \lambda \|\beta\|_1.$$

This optimization problem can be solved by each component:

$$(\hat{\beta}_n^{\text{lasso}})_j = \arg \min_{\beta} \left((\hat{\beta}_n)_j - \beta \right)^2 + \lambda \beta.$$

The gradient of objective function is

$$\frac{1}{2} \frac{\partial}{\partial \beta} = \beta - (\hat{\beta}_n)_j + \frac{\lambda}{2} \text{sgn}(\beta).$$

The solution is simply

$$(\hat{\beta}_n^{\text{lasso}})_j = \max(0, (\hat{\beta}_n)_j - \lambda/2).$$

Appendix-6

Our goal is to prove

$$\max_{\Delta \in M} \|\mathbb{Y} - (\mathbb{X} + \Delta)\beta\|_2 = \|\mathbb{Y} - \mathbb{X}\beta\|_2 + \sum_i c_i |\beta_i|$$

with $M = \left\{ \Delta \mid \sqrt{\sum_i \Delta_{i,j}^2} \leq c_j \right\}$. First note that from triangle inequality we have

$$\|\mathbb{Y} - (\mathbb{X} + \Delta)\beta\|_2 = \left\| \mathbb{Y} - \mathbb{X}\beta - \sum_i \Delta_i \beta_i \right\|_2 \leq \|\mathbb{Y} - \mathbb{X}\beta\|_2 + \sum_i c_i |\beta_i|.$$

To show there exists a Δ such that triangle equality holds, we simply choose a Δ such that $\Delta\beta$ is in the same direction of $\mathbb{Y} - \mathbb{X}\beta$. Therefore we finish the proof.